compiler/backend/stackLangScript.sml
@@ -37,6 +37,7 @@ val _ = Datatype `
        | While cmp num ('a reg_imm) stackLang$prog
        | JumpLower num num num (* reg, reg, target name *)
        | Alloc num
+       | StoreConsts
        | Raise num
        | Return num num
        | FFI string num num num num num (* FFI index, conf_ptr, conf_len,
@@ -84,7 +85,11 @@ val list_Seq_def = Define `
 
 val gc_stub_location_def = Define`
   gc_stub_location = stack_num_stubs-1`;
+val store_consts_stub_location_def = Define`
+  store_consts_stub_location = gc_stub_location-1`;
 val gc_stub_location_eq = save_thm("gc_stub_location_eq",
   gc_stub_location_def |> CONV_RULE(RAND_CONV EVAL));
+val store_consts_stub_location_eq = save_thm("store_consts_stub_location_eq",
+  store_consts_stub_location_def |> CONV_RULE(RAND_CONV EVAL));
 
 val _ = export_theory();
